WIP on finite sets examples
I can't seem to figure out how to make use of
ADTRefinementPreservesConstructors, because it seems to give me side
conditions that are unprovable in general.  (See comment labeled with
HELP.)

examples/FiniteSetsExamples.v
@@ -1,13 +1,23 @@
 (** * Some examples about dealing with finite sets *)
 Require Import Coq.Strings.String Coq.Sets.Ensembles Coq.Sets.Finite_sets Coq.Lists.List.
-Require Import ADT ADT.ComputationalADT ADTRefinement.Core ADTNotation ADTRefinement.GeneralRefinements.
+Require Import ADT ADT.ComputationalADT ADTRefinement.Core ADTNotation ADTRefinement.GeneralRefinements QueryStructure.IndexedEnsembles.
 
 Set Implicit Arguments.
 
 Local Open Scope string_scope.
 
 (** TODO: Figure out where Facade words live, and use that *)
-Definition word := nat.
+Module Type BedrockWordT.
+  Axiom W : Type.
+  Axiom wzero : W.
+  Axiom wplus : W -> W -> W.
+End BedrockWordT.
+
+Module Import BedrockWord : BedrockWordT.
+  Definition W := nat.
+  Definition wzero := 0.
+  Definition wplus := plus.
+End BedrockWord.
 
 (** We define the interface for finite sets *)
 (** QUESTION: Does Facade give us any other methods?  Do we want to
@@ -15,24 +25,24 @@ Definition word := nat.
 Definition FiniteSetSig : ADTSig :=
   ADTsignature {
       Constructor "Empty" : unit -> rep,
-      Method "Add" : rep x word -> rep x unit,
-      Method "Remove" : rep x word -> rep x unit,
-      Method "In" : rep x word -> rep x bool,
+      Method "Add" : rep x W -> rep x unit,
+      Method "Remove" : rep x W -> rep x unit,
+      Method "In" : rep x W -> rep x bool,
       Method "Size" : rep x unit -> rep x nat
     }.
 
 (** And now the spec *)
 Definition FiniteSetSpec : ADT FiniteSetSig :=
-  ADTRep (Ensemble word) {
+  ADTRep (Ensemble W) {
     Def Constructor "Empty" (_ : unit) : rep := ret (Empty_set _),
 
-    Def Method "Add" (xs : rep , x : word) : unit :=
+    Def Method "Add" (xs : rep , x : W) : unit :=
       ret (Add _ xs x, tt),
 
-    Def Method "Remove" (xs : rep , x : word) : unit :=
+    Def Method "Remove" (xs : rep , x : W) : unit :=
       ret (Subtract _ xs x, tt),
 
-    Def Method "In" (xs : rep , x : word) : bool :=
+    Def Method "In" (xs : rep , x : W) : bool :=
         (b <- { b : bool | b = true <-> Ensembles.In _ xs x };
          ret (xs, b)),
 
@@ -45,22 +55,21 @@ Definition FiniteSetSpec : ADT FiniteSetSig :=
 (** Now we spec out two examples, the count of the unique elements in
     a list, and the sum of the unique elements in a list. *)
 
-(** QUESTION: Do we want to start from [list]s?  From [Ensemble]s,
-    somehow?  (But then how do we end up with computations not
-    mentioning [Ensemble]s?)  Do we want to end up with something that
-    takes in a [list], or something else? *)
-
-Definition is_unique_list_of {T} (new orig : list T) : Prop
-  := NoDup new /\ (forall x, List.In x orig <-> List.In x new).
-
 (** QUESTION: Are these reasonable ways of specifying these specs? *)
 
-Definition countUniqueSpec (ls : list word) : Comp nat
-  := { n : nat | exists xs, is_unique_list_of xs ls /\ length xs = n }.
+Definition countUniqueSpec (ls : list W) : Comp nat
+  := (S <- { S : Ensemble W | forall x, Ensembles.In _ S x <-> List.In x ls  };
+      { n : nat | cardinal _ S n }).
 
-Definition sumUniqueSpec (ls : list word) : Comp word
-  := xs <- { xs : list word | is_unique_list_of xs ls };
-    ret (List.fold_right plus 0 xs).
+Definition countUniqueSpec' (ls : list W) : Comp nat
+  := (S <- { S : Ensemble W | forall x, Ensembles.In _ S x <-> List.In x ls  };
+      xs <- { ls' : list W | EnsembleListEquivalence S ls' };
+      ret (List.length xs)).
+
+Definition sumUniqueSpec (ls : list W) : Comp W
+  := (S <- { S : Ensemble W | forall x, Ensembles.In _ S x <-> List.In x ls };
+      xs <- { ls' : list W | EnsembleListEquivalence S ls' };
+      ret (List.fold_right wplus wzero xs)).
 
 Notation FullySharpenedComputation spec
   := { c : _ | refine spec (ret c) }%type.
@@ -77,7 +86,128 @@ Notation FullySharpenedComputation spec
 (** QUESTION: Did I get the right target implementation that we want
     the tactics to find in the following two examples? *)
 
-Definition countUniqueImpl (FiniteSetImpl : FullySharpened FiniteSetSpec) (ls : list word)
+(*Lemma cardinal_to_list {T} (S : Ensemble T)
+: refineEquiv { n : nat | cardinal _ S n }
+              (xs <- { ls : list T | EnsembleListEquivalence S ls };
+               ret (length xs)).
+  *)
+(** We prove equivalences to handle various operations on ensembles,
+    and on lists equivalent to ensembles. *)
+Section FiniteSetHelpers.
+  Context (FiniteSetImpl : FullySharpened FiniteSetSpec).
+
+  Local Hint Extern 0 =>
+  match goal with
+    | [ H : False |- _ ] => destruct H
+  end.
+  Local Hint Extern 0 => apply Constructive_sets.Noone_in_empty.
+  Local Hint Resolve Constructive_sets.Add_intro2 Constructive_sets.Add_intro1.
+
+  Definition FiniteSetOfList (ls : list W) : cRep (projT1 FiniteSetImpl)
+    := List.fold_right
+         (fun w xs => fst (CallMethod (projT1 FiniteSetImpl) "Add" xs w))
+         (CallConstructor (projT1 FiniteSetImpl) "Empty" tt)
+         ls.
+
+  Definition EnsembleOfList {T} (ls : list T) : Ensemble T
+    := List.fold_right
+         (fun w xs => Ensembles.Add _ xs w)
+         (Ensembles.Empty_set _)
+         ls.
+
+  Lemma EnsembleOfList_In {T} (ls : list T)
+  : forall x, Ensembles.In _ (EnsembleOfList ls) x <-> In x ls.
+  Proof.
+    induction ls;
+    repeat match goal with
+             | _ => split
+             | _ => progress split_iff
+             | [ H : Ensembles.In _ (Ensembles.Add _ _ _) _ |- _ ] => apply Constructive_sets.Add_inv in H
+             | [ H : Ensembles.In _ (Empty_set _) _ |- _ ] => apply Constructive_sets.Noone_in_empty in H
+             | _ => progress destruct_head or
+             | _ => intro
+             | _ => progress subst
+             | _ => progress simpl in *
+             | _ => solve [ eauto ]
+             | _ => solve [ right; eauto ]
+             | _ => left; reflexivity
+           end.
+  Qed.
+
+  (*Lemma EnsembleOfList_FiniteSetOfList ls
+  : AbsR (projT2 FiniteSetImpl) (EnsembleOfList ls) (FiniteSetOfList ls).
+  Proof.
+    unfold EnsembleOfList, FiniteSetOfList;
+    induction ls; simpl.
+    Set Printing Coercions.
+    lazymatch goal with
+      | [ |- context[CallConstructor (projT1 ?impl) ?idx ?arg] ]
+        => idtac;
+          let lem := constr:(ADTRefinementPreservesConstructors (projT2 impl) {| bindex := idx |} arg) in
+           pose proof lem; simpl in *
+    end.
+    hnf in H.
+
+    *)
+
+  Lemma comp_split_snd {A B} (x : A * B)
+  : refineEquiv (ret (snd x))
+                (ab <- ret x;
+                 ret (snd ab)).
+  Proof.
+    autorewrite with refine_monad; reflexivity.
+  Qed.
+
+  Lemma refine_skip {A B C} (c : Comp A) (f : A -> Comp B) (dummy : A -> Comp C)
+  : refine (Bind c f)
+           (a <- c;
+            dummy a;;
+                  f a).
+  Proof.
+    repeat first [ intro
+                 | inversion_by computes_to_inv
+                 | econstructor; eassumption
+                 | econstructor; try eassumption; [] ].
+  Qed.
+
+  Ltac handle_calls :=
+    repeat match goal with
+             | [ |- context[ret ((CallMethod (projT1 ?impl) ?idx) ?rep ?arg)] ]
+               => let lem := constr:(fun rep' => ADTRefinementPreservesMethods (projT2 impl) {| bindex := idx |} rep' rep arg) in
+                  simpl rewrite <- lem
+             | [ |- context[ret ((CallConstructor (projT1 ?impl) ?idx) ?arg)] ]
+               => let lem := constr:(ADTRefinementPreservesConstructors (projT2 impl) {| bindex := idx |} arg) in
+                  simpl rewrite <- lem
+           end.
+
+  Lemma finite_set_handle_cardinal (ls : list W)
+  : refine (S <- { S : Ensemble W | forall x, Ensembles.In _ S x <-> List.In x ls  };
+            { n : nat | cardinal _ S n })
+           (ret (snd (CallMethod (projT1 FiniteSetImpl) "Size"
+                                 (FiniteSetOfList ls)
+                                 tt))).
+  Proof.
+    etransitivity; [ | apply comp_split_snd ].
+    handle_calls.
+    repeat first [ progress simpl
+                 | rewrite <- refine_skip
+                 | autosetoid_rewrite with refine_monad ].
+    instantiate (1 := EnsembleOfList ls).
+    { repeat intro.
+      econstructor; try eassumption; [].
+      inversion_by computes_to_inv.
+      constructor.
+      apply EnsembleOfList_In. }
+    { (** HELP: How can I prove this?  It seems false, if, e.g.,
+          [FiniteSetImpl] decides to use [False] as it's
+          representation.  But if this is unprovable, then
+          [ADTRefinementPreservesConstructors] seems utterly
+          useless. *)
+      admit. }
+  Qed.
+End FiniteSetHelpers.
+
+Definition countUniqueImpl (FiniteSetImpl : FullySharpened FiniteSetSpec) (ls : list W)
 : FullySharpenedComputation (countUniqueSpec ls).
 Proof.
   (** We turn the list into a finite set, and then call 'size' *)
@@ -92,7 +222,7 @@ Defined.
 
 (** And now we do the same for summing. *)
 
-Definition sumUniqueImpl (FiniteSetImpl : FullySharpened FiniteSetSpec) (ls : list word)
+Definition sumUniqueImpl (FiniteSetImpl : FullySharpened FiniteSetSpec) (ls : list W)
 : FullySharpenedComputation (sumUniqueSpec ls).
 Proof.
   (** We fold over the list, using a finite set to keep track of what
@@ -106,9 +236,9 @@ Proof.
                     if (snd (CallMethod (projT1 FiniteSetImpl) "In" xs w) : bool)
                     then xs_sum
                     else (fst (CallMethod (projT1 FiniteSetImpl) "Add" xs w),
-                          acc + w))
+                          wplus acc w))
                  (CallConstructor (projT1 FiniteSetImpl) "Empty" tt,
-                  0)
+                  wzero)
                  ls)).
   admit.
 Defined.
